one step further

Refine_Imperative_HOL/IICF/Impl/IICF_Array_Matrix.thy
@@ -30,15 +30,19 @@ begin
   (*definition "mtx_new N M c \<equiv> do {
     Array.make (N*M) (\<lambda>i. c (i div M, i mod M))
   }"*)
-  
+
+
+partial_function (heap) imp_for' :: "nat \<Rightarrow> nat \<Rightarrow> (nat \<Rightarrow> 'a \<Rightarrow> 'a Heap) \<Rightarrow> 'a \<Rightarrow> 'a Heap" where
+  "imp_for' i u f s = (if i \<ge> u then return s else f i s \<bind> imp_for' (i + 1) u f)"
+
   definition "mtx_tabulate N M c \<equiv> do {
     m \<leftarrow> Array.new (N*M) 0;
-  (*  (_,_,m) \<leftarrow> imp_for' 0 (N*M) (\<lambda>k (i,j,m). do {
+    (_,_,m) \<leftarrow> imp_for' 0 (N*M) (\<lambda>k (i,j,m). do {
       Array.upd k (c (i,j)) m;
       let j=j+1;
       if j<M then return (i,j,m)
       else return (i+1,0,m)
-    }) (0,0,m); *)
+    }) (0,0,m); 
     return m
   }"
       
@@ -64,16 +68,19 @@ begin
       using \<open>\<lbrakk>j < M; j' < M; i * M + j = i' * M + j'\<rbrakk> \<Longrightarrow> i = i'\<close> by auto  
     done
       
-  (*lemma mtx_index_unique[simp]: "\<lbrakk>i<(N::nat); j<M; i'<N; j'<M\<rbrakk> \<Longrightarrow> i*M+j = i'*M+j' \<longleftrightarrow> i=i' \<and> j=j'"
-    by (metis ab_semigroup_add_class.add.commute add_diff_cancel_right' div_if div_mult_self3 gr0I not_less0)*)
+  lemma mtx_index_unique[simp]: "\<lbrakk>i<(N::nat); j<M; i'<N; j'<M\<rbrakk> \<Longrightarrow> i*M+j = i'*M+j' \<longleftrightarrow> i=i' \<and> j=j'"
+    by (metis ab_semigroup_add_class.add.commute add_diff_cancel_right' div_if div_mult_self3 gr0I not_less0)
+
+declare [[print_trace]]
 (*
   lemma mtx_tabulate_rl[sep_heap_rules]:
     assumes NONZ: "mtx_nonzero c \<subseteq> {0..<N}\<times>{0..<M}"
-    shows "<emp> mtx_tabulate N M c <IICF_Array_Matrix.is_amtx N M c>"
+    shows "<timeCredit_assn (N*M*10+1)> mtx_tabulate N M c <IICF_Array_Matrix.is_amtx N M c>"
   proof (cases "M=0")
     case True thus ?thesis
       unfolding mtx_tabulate_def  
       using mtx_nonzeroD[OF _ NONZ]  
+      apply simp apply auto2
       by (sep_auto simp: is_amtx_def)
   next
     case False hence M_POS: "0<M" by auto
@@ -334,26 +341,36 @@ lemma mop_matrix_get_rule[sepref_fr_rules]:
   sepref_decl_impl amtx_copy: mtx_copy_aref .
    *) 
   definition [simp]: "op_amtx_new (N::nat) (M::nat) \<equiv> op_mtx_new"  
-  lemma amtx_fold_custom_new:
+(*  lemma amtx_fold_custom_new:
     "op_mtx_new \<equiv> op_amtx_new N M"
     apply simp done
- (*
+ 
     "mop_mtx_new \<equiv> \<lambda>c. RETURN (op_amtx_new N M c)"
     by (auto simp: mop_mtx_new_alt[abs_def]) *)
 
 
 
-  context fixes N M :: nat begin  
-    sepref_register "PR_CONST (op_amtx_new N M)" :: "(nat \<times> nat \<Rightarrow> 'a) \<Rightarrow> 'a i_mtx"
+context fixes N M :: nat begin
+
+    definition "mop_amtx_new = (%c. RETURNT (op_amtx_new N M c))"
+    sepref_register "mop_amtx_new"
+
+
   end
+                      
+  term mop_amtx_new
 
   lemma amtx_new_hnr[sepref_fr_rules]: 
     fixes A :: "'a::zero \<Rightarrow> 'b::{zero,heap} \<Rightarrow> assn"
     shows "CONSTRAINT (IS_PURE PRES_ZERO_UNIQUE) A \<Longrightarrow>
-    (mtx_tabulate N M, (RETURNT \<circ> PR_CONST (op_amtx_new N M)))
+    (mtx_tabulate N M, ( PR_CONST (mop_amtx_new N M)))
     \<in> [\<lambda>x. mtx_nonzero x \<subseteq> {0..<N} \<times> {0..<M}]\<^sub>a (pure (nat_rel \<times>\<^sub>r nat_rel \<rightarrow> the_pure A))\<^sup>k \<rightarrow> amtx_assn N M A"
    (* using amtx_new_by_tab_hnr[of A N M] by simp *) sorry
   
+
+lemma amtx_fold_custom_new:
+    "\<And>c. RETURNT (op_mtx_new c) =  mop_amtx_new N M c" by(auto simp: mop_amtx_new_def)
+
 
 (*
   lemma [def_pat_rules]: "op_amtx_new$N$M \<equiv> UNPROTECT (op_amtx_new N M)" by simp
